examples/Debug/go.sh
@@ -1,23 +1,37 @@
-# usage: ./go.sh
+# usage:
+# ./go.sh
+# ./go.sh mlv
+
+
+ARG=$1
+if [[ ${ARG} = "" ]]; then
+  ARG="Debug_ml.vo"
+fi
+
 
 # For development purposes
 # make sure to first recompile your local TLC
 
 make -C ../../generator
 make -f Makefile.dev _CoqProject
-make -C ../../lib/coq -f Makefile.dev depend
-make -j4 -C ../../lib/coq -f Makefile.dev
-make -C ../../lib/stdlib -f Makefile.dev depend
-make -j4 -C ../../lib/stdlib -f Makefile.dev
-make -f Makefile.dev depend
 
-ARG=$1
-if [[ ${ARG} = "" ]]; then
-  ARG="Debug_ml.vo"
+if [[ ${ARG} = "mlv" ]]; then
+
+  make -C ../../lib/stdlib -f Makefile.dev depend
+  make -j4 -C ../../lib/stdlib -f Makefile.dev Pervasives_ml.v
+  make -f Makefile.dev ${ARG}
+
+else
+
+  make -C ../../lib/coq -f Makefile.dev depend
+  make -j4 -C ../../lib/coq -f Makefile.dev
+  make -C ../../lib/stdlib -f Makefile.dev depend
+  make -j4 -C ../../lib/stdlib -f Makefile.dev
+  make -f Makefile.dev depend
+
+  make -f Makefile.dev ${ARG}
+
 fi
-make -f Makefile.dev ${ARG}
 
-# only for generation:
-# ./go.sh Debug_ml.v
 
 #coqide Debug_ml.v Debug_proof.v
